Fix some minor regressions due to recent [equiv_states] changes

vale/code/lib/transformers/Vale.Transformers.InstructionReorder.fst
@@ -361,6 +361,8 @@ let rec lemma_instr_apply_eval_inouts_equiv_states
     | Some v ->
       lemma_instr_apply_eval_inouts_equiv_states outs inouts args (f v) oprs s1 s2
 
+#push-options "--z3rlimit 10 --max_fuel 1 --max_ifuel 0"
+
 let lemma_instr_write_output_implicit_equiv_states
     (i:instr_operand_implicit) (v:instr_val_t (IOpIm i))
     (s_orig1 s1 s_orig2 s2:machine_state) :
@@ -372,9 +374,28 @@ let lemma_instr_write_output_implicit_equiv_states
         (equiv_states
            (instr_write_output_implicit i v s_orig1 s1)
            (instr_write_output_implicit i v s_orig2 s2)))) =
-  assert (equiv_states_ext
-            (instr_write_output_implicit i v s_orig1 s1)
-            (instr_write_output_implicit i v s_orig2 s2))
+  let snew1, snew2 =
+    (instr_write_output_implicit i v s_orig1 s1),
+    (instr_write_output_implicit i v s_orig2 s2) in
+  assert (equiv_states_ext snew1 snew2) (* OBSERVE *)
+
+let lemma_instr_write_output_explicit_equiv_states
+    (i:instr_operand_explicit) (v:instr_val_t (IOpEx i)) (o:instr_operand_t i)
+    (s_orig1 s1 s_orig2 s2:machine_state) :
+  Lemma
+    (requires (
+        (equiv_states s_orig1 s_orig2) /\
+        (equiv_states s1 s2)))
+    (ensures (
+        (equiv_states
+           (instr_write_output_explicit i v o s_orig1 s1)
+           (instr_write_output_explicit i v o s_orig2 s2)))) =
+  let snew1, snew2 =
+    (instr_write_output_explicit i v o s_orig1 s1),
+    (instr_write_output_explicit i v o s_orig2 s2) in
+  assert (equiv_states_ext snew1 snew2) (* OBSERVE *)
+
+#pop-options
 
 let rec lemma_instr_write_outputs_equiv_states
     (outs:list instr_out) (args:list instr_operand)
@@ -401,9 +422,9 @@ let rec lemma_instr_write_outputs_equiv_states
       match i with
       | IOpEx i ->
         let oprs = coerce oprs in
+        lemma_instr_write_output_explicit_equiv_states i v (fst oprs) s_orig1 s1 s_orig2 s2;
         let s1 = instr_write_output_explicit i v (fst oprs) s_orig1 s1 in
         let s2 = instr_write_output_explicit i v (fst oprs) s_orig2 s2 in
-        assert (equiv_states_ext s1 s2);
         lemma_instr_write_outputs_equiv_states outs args vs (snd oprs) s_orig1 s1 s_orig2 s2
       | IOpIm i ->
         lemma_instr_write_output_implicit_equiv_states i v s_orig1 s1 s_orig2 s2;
